Rename clos_inlineXX theories to clos_knownXX

compiler/backend/clos_knownScript.sml
@@ -1,10 +1,225 @@
 open preamble closLangTheory;
+open db_varsTheory;
 
 val _ = new_theory "clos_known";
 
-val _ = set_grammar_ancestry ["closLang", "sptree", "misc"]
+(* val _ = set_grammar_ancestry ["closLang", "sptree", "misc", "backend_common"] *)
 
 val _ = patternMatchesLib.ENABLE_PMATCH_CASES();
+
+(* This definition is written to exit as soon as possible. *)
+val is_small_aux_def = tDefine "is_small_aux" `
+  (is_small_aux n [] = n) /\
+  (is_small_aux n (x::y::xs) =
+     if n = 0n then n else
+       let n = is_small_aux n [x] in if n = 0 then n else
+         is_small_aux n (y::xs)) /\
+  (is_small_aux n [Var t v] = n) /\
+  (is_small_aux n [If t x1 x2 x3] =
+     let n = n - 1 in if n = 0 then 0 else
+     let n = is_small_aux n [x1] in if n = 0 then 0 else
+     let n = is_small_aux n [x2] in if n = 0 then 0 else
+       is_small_aux n [x3]) /\
+  (is_small_aux n [Let t xs x2] =
+     let n = n - 1 in if n = 0 then 0 else
+     let n = is_small_aux n xs in if n = 0 then 0 else
+       is_small_aux n [x2]) /\
+  (is_small_aux n [Raise t x1] =
+     let n = n - 1 in if n = 0 then 0 else
+       is_small_aux n [x1]) /\
+  (is_small_aux n [Handle t x1 x2] =
+     let n = n - 1 in if n = 0 then 0 else
+     let n = is_small_aux n [x1] in if n = 0 then 0 else
+       is_small_aux n [x2]) /\
+  (is_small_aux n [Op t op xs] =
+     let n = n - 1 in if n = 0 then 0 else
+       is_small_aux n xs) /\
+  (is_small_aux n [Tick t x] = is_small_aux n [x]) /\
+  (is_small_aux n [Call t ticks dest xs] =
+     let n = n - 1 in if n = 0 then 0 else
+       is_small_aux n xs) /\
+  (is_small_aux n [Fn t loc_opt ws_opt num_args x1] =
+     let n = n - 1 in if n = 0 then 0 else
+       is_small_aux n [x1]) /\
+  (is_small_aux n [Letrec t loc_opt ws_opt fns x1] =
+     let n = n - 1 in if n = 0 then 0 else
+     let n = is_small_aux n (MAP SND fns) in if n = 0 then 0 else
+       is_small_aux n [x1]) /\
+  (is_small_aux n [App t loc_opt x1 xs] =
+     let n = n - 1 in if n = 0 then 0 else
+     let n = is_small_aux n [x1] in if n = 0 then 0 else
+       is_small_aux n xs)`
+  (WF_REL_TAC `measure (exp3_size o SND)`
+   \\ simp [] \\ rpt strip_tac
+   \\ `exp3_size (MAP SND fns) <= exp1_size fns`
+      by (Induct_on `fns` \\ simp [exp_size_def] \\ Cases \\ simp [exp_size_def])
+   \\ simp []);
+
+val is_small_def = Define `
+  is_small limit e = ~(is_small_aux limit [e] = 0)`;
+
+val is_rec_def = tDefine "is_rec" `
+  (is_rec n [] = F) /\
+  (is_rec n (x::y::xs) =
+     if is_rec n [x] then T else
+       is_rec n (y::xs)) /\
+  (is_rec n [Var t v] = F) /\
+  (is_rec n [If t x1 x2 x3] =
+     if is_rec n [x1] then T else
+     if is_rec n [x2] then T else
+       is_rec n [x3]) /\
+  (is_rec n [Let t xs x2] =
+     if is_rec n xs then T else
+       is_rec n [x2]) /\
+  (is_rec n [Raise t x1] = is_rec n [x1]) /\
+  (is_rec n [Handle t x1 x2] =
+     if is_rec n [x1] then T else
+       is_rec n [x2]) /\
+  (is_rec n [Op t op xs] = is_rec n xs) /\
+  (is_rec n [Tick t x] = is_rec n [x]) /\
+  (is_rec n [Call t ticks dest xs] = is_rec n xs) /\
+  (is_rec n [Fn t loc_opt ws_opt num_args x1] =
+     is_rec n [x1]) /\
+  (is_rec n [Letrec t loc_opt ws_opt fns x1] =
+     if is_rec n (MAP SND fns) then T else
+       is_rec n [x1]) /\
+  (is_rec n [App t loc_opt x1 xs] =
+     if loc_opt = SOME n then T else
+     if is_rec n [x1] then T else
+       is_rec n xs)`
+  (WF_REL_TAC `measure (exp3_size o SND)`
+   \\ simp [] \\ rpt strip_tac
+   \\ `exp3_size (MAP SND fns) <= exp1_size fns`
+      by (Induct_on `fns` \\ simp [exp_size_def] \\ Cases \\ simp [exp_size_def])
+   \\ simp []);
+
+val free_def = tDefine "free" `
+  (free [] = ([],Empty)) /\
+  (free ((x:closLang$exp)::y::xs) =
+     let (c1,l1) = free [x] in
+     let (c2,l2) = free (y::xs) in
+       (c1 ++ c2,mk_Union l1 l2)) /\
+  (free [Var t v] = ([Var t v], Var v)) /\
+  (free [If t x1 x2 x3] =
+     let (c1,l1) = free [x1] in
+     let (c2,l2) = free [x2] in
+     let (c3,l3) = free [x3] in
+       ([If t (HD c1) (HD c2) (HD c3)],mk_Union l1 (mk_Union l2 l3))) /\
+  (free [Let t xs x2] =
+     let (c1,l1) = free xs in
+     let (c2,l2) = free [x2] in
+       ([Let t c1 (HD c2)],mk_Union l1 (Shift (LENGTH xs) l2))) /\
+  (free [Raise t x1] =
+     let (c1,l1) = free [x1] in
+       ([Raise t (HD c1)],l1)) /\
+  (free [Tick t x1] =
+     let (c1,l1) = free [x1] in
+       ([Tick t (HD c1)],l1)) /\
+  (free [Op t op xs] =
+     let (c1,l1) = free xs in
+       ([Op t op c1],l1)) /\
+  (free [App t loc_opt x1 xs2] =
+     let (c1,l1) = free [x1] in
+     let (c2,l2) = free xs2 in
+       ([App t loc_opt (HD c1) c2],mk_Union l1 l2)) /\
+  (free [Fn t loc _ num_args x1] =
+     let (c1,l1) = free [x1] in
+     let l2 = Shift num_args l1 in
+       ([Fn t loc (SOME (vars_to_list l2)) num_args (HD c1)],l2)) /\
+  (free [Letrec t loc _ fns x1] =
+     let m = LENGTH fns in
+     let res = MAP (\(n,x). let (c,l) = free [x] in
+                              ((n,HD c),Shift (n + m) l)) fns in
+     let c1 = MAP FST res in
+     let l1 = list_mk_Union (MAP SND res) in
+     let (c2,l2) = free [x1] in
+       ([Letrec t loc (SOME (vars_to_list l1)) c1 (HD c2)],
+        mk_Union l1 (Shift (LENGTH fns) l2))) /\
+  (free [Handle t x1 x2] =
+     let (c1,l1) = free [x1] in
+     let (c2,l2) = free [x2] in
+       ([Handle t (HD c1) (HD c2)],mk_Union l1 (Shift 1 l2))) /\
+  (free [Call t ticks dest xs] =
+     let (c1,l1) = free xs in
+       ([Call t ticks dest c1],l1))`
+ (WF_REL_TAC `measure exp3_size`
+  \\ REPEAT STRIP_TAC \\ IMP_RES_TAC exp1_size_lemma \\ DECIDE_TAC);
+
+val free_ind = theorem "free_ind";
+
+(*
+val free_LENGTH_LEMMA = Q.prove(
+  `!xs. (case free xs of (ys,s1) => (LENGTH xs = LENGTH ys))`,
+  recInduct free_ind \\ REPEAT STRIP_TAC
+  \\ FULL_SIMP_TAC (srw_ss()) [free_def]
+  \\ SRW_TAC [] [] \\ SRW_TAC [] []
+  \\ REPEAT BasicProvers.FULL_CASE_TAC \\ FULL_SIMP_TAC (srw_ss()) []
+  \\ REV_FULL_SIMP_TAC std_ss [] \\ FULL_SIMP_TAC (srw_ss()) []
+  \\ SRW_TAC [] [] \\ DECIDE_TAC)
+  |> SIMP_RULE std_ss [] |> SPEC_ALL;
+
+val free_LENGTH = Q.store_thm("free_LENGTH",
+  `!xs ys l. (free xs = (ys,l)) ==> (LENGTH ys = LENGTH xs)`,
+  REPEAT STRIP_TAC \\ MP_TAC free_LENGTH_LEMMA \\ fs []);
+
+val free_SING = Q.store_thm("free_SING",
+  `(free [x] = (ys,l)) ==> ?y. ys = [y]`,
+  REPEAT STRIP_TAC \\ IMP_RES_TAC free_LENGTH
+  \\ Cases_on `ys` \\ fs [LENGTH_NIL]);
+
+val LENGTH_FST_free = Q.store_thm("LENGTH_FST_free",
+  `LENGTH (FST (free fns)) = LENGTH fns`,
+  Cases_on `free fns` \\ fs [] \\ IMP_RES_TAC free_LENGTH);
+
+val HD_FST_free = Q.store_thm("HD_FST_free",
+  `[HD (FST (free [x1]))] = FST (free [x1])`,
+  Cases_on `free [x1]` \\ fs []
+  \\ imp_res_tac free_SING \\ fs[]);
+
+val free_CONS = Q.store_thm("free_CONS",
+  `FST (free (x::xs)) = HD (FST (free [x])) :: FST (free xs)`,
+  Cases_on `xs` \\ fs [free_def,SING_HD,LENGTH_FST_free,LET_DEF]
+  \\ Cases_on `free [x]` \\ fs []
+  \\ Cases_on `free (h::t)` \\ fs [SING_HD]
+\\ IMP_RES_TAC free_SING \\ fs []);
+*)
+
+val closed_def = Define `
+  closed x = isEmpty (db_to_set (SND (free [x])))`
+
+val contains_closures_def = tDefine "contains_closures" `
+  (contains_closures [] = F) /\
+  (contains_closures (x::y::xs) =
+    if contains_closures [x] then T else
+      contains_closures (y::xs)) /\
+  (contains_closures [Var t v] = F) /\
+  (contains_closures [If t x1 x2 x3] =
+     if contains_closures [x1] then T else
+     if contains_closures [x2] then T else
+       contains_closures [x3]) /\
+  (contains_closures [Let t xs x2] =
+     if contains_closures xs then T else
+       contains_closures [x2]) /\
+  (contains_closures [Raise t x1] = contains_closures [x1]) /\
+  (contains_closures [Handle t x1 x2] =
+     if contains_closures [x1] then T else
+       contains_closures [x2]) /\
+  (contains_closures [Op t op xs] = contains_closures xs) /\
+  (contains_closures [Tick t x] = contains_closures [x]) /\
+  (contains_closures [Call t ticks dest xs] = contains_closures xs) /\
+  (contains_closures [Fn t loc_opt ws_opt num_args x1] = T) /\
+  (contains_closures [Letrec t loc_opt ws_opt fns x1] = T) /\
+  (contains_closures [App t loc_opt x1 xs] =
+     if contains_closures [x1] then T else
+       contains_closures xs)`
+  (wf_rel_tac `measure exp3_size`);
+
+val must_inline_def = Define `
+  must_inline limit name num_args e =
+    if ~(is_small limit e) then F else
+    if is_rec name [e] then F else
+    if contains_closures [e] then F else
+    closed (Fn None NONE NONE num_args e)`
 
 (* -----------------------------------------------------------------
 
@@ -22,7 +237,7 @@ val _ = patternMatchesLib.ENABLE_PMATCH_CASES();
 
 val _ = Datatype `
   val_approx =
-    Clos num num                (* location in code table, arity *)
+    Clos num num (exp option)     (* location in code table, arity, function body *)
   | Tuple num (val_approx list) (* conses or tuples *)
   | Int int                     (* used to index tuples *)
   | Other                       (* unknown *)
@@ -35,7 +250,7 @@ val merge_def = tDefine "merge" `
   (merge (Tuple tg1 xs) (Tuple tg2 ys) =
      if LENGTH xs = LENGTH ys ∧ tg1 = tg2 then Tuple tg1 (MAP2 merge xs ys)
      else Other) ∧
-  (merge (Clos m1 n1) (Clos m2 n2) = if m1 = m2 ∧ n1 = n2 then Clos m1 n1
+  (merge (Clos m1 n1 e1) (Clos m2 n2 e2) = if m1 = m2 ∧ n1 = n2 /\ e1 = e2 then Clos m1 n1 e1
                                      else Other) ∧
   (merge (Int i) (Int j) = if i = j then Int i else Other) ∧
   (merge _ _ = Other)
@@ -57,7 +272,7 @@ val merge_tup_def = tDefine "merge_tup" `
      if LENGTH xs = LENGTH ys ∧ tg1 = tg2 then
        Tuple tg1 (MAP merge_tup (ZIP(xs,ys)))
      else Other) ∧
-  (merge_tup (Clos m1 n1,Clos m2 n2) = if m1 = m2 ∧ n1 = n2 then Clos m1 n1
+  (merge_tup (Clos m1 n1 e1,Clos m2 n2 e2) = if m1 = m2 ∧ n1 = n2 /\ e1 = e2 then Clos m1 n1 e1
                                      else Other) ∧
   (merge_tup (Int i,Int j) = if i = j then Int i else Other) ∧
   (merge_tup (_,_) = Other)
@@ -105,8 +320,8 @@ val known_op_def = Define `
      | [] => (Other,g)
      | (a::xs) =>
        dtcase lookup n g of
-       | NONE => (Other,insert n a g)
-       | SOME other => (Other,insert n (merge other a) g)) /\
+       | NONE => (Other, insert n a g)
+       | SOME other => (Other, insert n (merge other a) g)) /\
   (known_op (Cons tg) as g = (Tuple tg as,g)) /\
   (known_op (Const i) as g = (Int i,g)) /\
   (known_op El as g =
@@ -133,9 +348,9 @@ known_op op as g =
     (case as of
      | [] => (Other,g)
      | (a::xs) =>
-       case lookup n g of
-       | NONE => (Other,insert n a g)
-       | SOME other => (Other,insert n (merge other a) g))
+       dtcase lookup n g of
+       | NONE => (Other, insert n a g)
+       | SOME other => (Other, insert n (merge other a) g))
   | Cons tg => (Tuple tg as,g)
   | Const i => (Int i,g)
   | El =>
@@ -157,20 +372,33 @@ val EL_MEM_LEMMA = Q.prove(
   Induct \\ fs [] \\ REPEAT STRIP_TAC \\ Cases_on `i` \\ fs []);
 
 val dest_Clos_def = Define `
-  (dest_Clos (Clos n a) = SOME (n,a)) /\
+  (dest_Clos (Clos n a e) = SOME (n,a,e)) /\
   (dest_Clos _ = NONE)`;
 val _ = export_rewrites["dest_Clos_def"];
 
-val clos_gen_def = Define`
-  (clos_gen n i [] = []) ∧
-  (clos_gen n i ((x,_)::xs) = Clos (n+2*i) x::clos_gen n (i+1) xs)`
+val clos_approx_def = Define `
+  clos_approx limit loc num_args body =
+    Clos loc num_args (if must_inline limit loc num_args body
+                       then SOME body else NONE)`;
 
-val _ = Datatype`globalOpt = gO_Int int | gO_NullTuple num | gO_None`
+(*
+val clos_gen_def = Define`
+  (clos_gen limit n i [] = []) ∧
+  (clos_gen limit n i ((a,e)::xs) =
+    clos_approx limit (n+2*i) a e::clos_gen limit n (i+1) xs)`;
+*)
+
+val clos_gen_noinline_def = Define`
+  (clos_gen_noinline n i [] = []) /\
+  (clos_gen_noinline n i ((a,e)::xs) =
+    Clos (n+2*i) a NONE::clos_gen_noinline n (i+1) xs)`;
+
+val _ = Datatype `globalOpt = gO_Int int | gO_NullTuple num | gO_None`
 
 val isGlobal_def = Define`
   (isGlobal (Global _) ⇔ T) ∧
-  (isGlobal _ ⇔ F)
-`
+  (isGlobal _ ⇔ F)`;
+
 val isGlobal_pmatch = Q.store_thm("isGlobal_pmatch",`!op.
   isGlobal op =
   case op of
@@ -184,138 +412,281 @@ val gO_destApx_def = Define`
   (gO_destApx (Int i) = gO_Int i) ∧
   (gO_destApx (Tuple tag args) = if NULL args then gO_NullTuple tag
                                  else gO_None) ∧
-  (gO_destApx _ = gO_None)
-`;
+  (gO_destApx _ = gO_None)`;
+
+val mk_Ticks_def = Define `
+  (mk_Ticks t tc 0 e = e) /\
+  (mk_Ticks t tc (SUC n) e = Tick (t§tc) (mk_Ticks t (tc + 1) n e))`;
+
+(* Accessors for the limit structure *)
+val size_limit_def = Define `size_limit = FST`;
+val depth_limit_def = Define `depth_limit = SND`;
+val dec_depth_def = Define `dec_depth = (I ## \d. d - 1n)`;
 
 val known_def = tDefine "known" `
-  (known [] vs (g:val_approx spt) = ([],g)) /\
-  (known ((x:closLang$exp)::y::xs) vs g =
-     let (e1,g) = known [x] vs g in
-     let (e2,g) = known (y::xs) vs g in
-       (e1 ++ e2,g)) /\
-  (known [Var t v] vs g =
+  (known limit [] vs (g:val_approx spt) = ([],g)) /\
+  (known limit ((x:closLang$exp)::y::xs) vs g =
+     let (eas1,g) = known limit [x] vs g in
+     let (eas2,g) = known limit (y::xs) vs g in
+       (eas1 ++ eas2,g)) /\
+  (known limit [Var t v] vs g =
      ([(Var t v,any_el v vs Other)],g)) /\
-  (known [If t x1 x2 x3] vs g =
-     let (e1,g) = known [x1] vs g in
-     let (e2,g) = known [x2] vs g in
-     let (e3,g) = known [x3] vs g in
-     let (e1,a1) = HD e1 in
-     let (e2,a2) = HD e2 in
-     let (e3,a3) = HD e3 in
+  (known limit [If t x1 x2 x3] vs g =
+     let (ea1,g) = known limit [x1] vs g in
+     let (ea2,g) = known limit [x2] vs g in
+     let (ea3,g) = known limit [x3] vs g in
+     let (e1,a1) = HD ea1 in
+     let (e2,a2) = HD ea2 in
+     let (e3,a3) = HD ea3 in
        ([(If t e1 e2 e3), merge a2 a3],g)) /\
-  (known [Let t xs x2] vs g =
-     let (e1,g) = known xs vs g in
-     let (e2,g) = known [x2] (MAP SND e1 ++ vs) g in
-     let (e2,a2) = HD e2 in
-       ([(Let t (MAP FST e1) e2, a2)],g)) /\
-  (known [Raise t x1] vs g =
-     let (e1,g) = known [x1] vs g in
-     let (e1,a1) = HD e1 in
+  (known limit [Let t xs x2] vs g =
+     let (ea1,g) = known limit xs vs g in
+     let (ea2,g) = known limit [x2] (MAP SND ea1 ++ vs) g in
+     let (e2,a2) = HD ea2 in
+       ([(Let t (MAP FST ea1) e2, a2)],g)) /\
+  (known limit [Raise t x1] vs g =
+     let (ea1,g) = known limit [x1] vs g in
+     let (e1,a1) = HD ea1 in
        ([(Raise t e1,Impossible)],g)) /\
-  (known [Tick t x1] vs g =
-     let (e1,g) = known [x1] vs g in
-     let (e1,a1) = HD e1 in
+  (known limit [Tick t x1] vs g =
+     let (ea1,g) = known limit [x1] vs g in
+     let (e1,a1) = HD ea1 in
        ([(Tick t e1,a1)],g)) /\
-  (known [Handle t x1 x2] vs g =
-     let (e1,g) = known [x1] vs g in
-     let (e2,g) = known [x2] (Other::vs) g in
-     let (e1,a1) = HD e1 in
-     let (e2,a2) = HD e2 in
+  (known limit [Handle t x1 x2] vs g =
+     let (ea1,g) = known limit [x1] vs g in
+     let (ea2,g) = known limit [x2] (Other::vs) g in
+     let (e1,a1) = HD ea1 in
+     let (e2,a2) = HD ea2 in
        ([(Handle t e1 e2,merge a1 a2)],g)) /\
-  (known [Call t ticks dest xs] vs g =
-     let (e1,g) = known xs vs g in
-       ([(Call t ticks dest (MAP FST e1),Other)],g)) /\
-  (known [Op t op xs] vs g =
-     let (e1,g) = known xs vs g in
-     let (a,g) = known_op op (REVERSE (MAP SND e1)) g in
+  (known limit [Call t ticks dest xs] vs g =
+     let (ea1,g) = known limit xs vs g in
+       ([(Call t ticks dest (MAP FST ea1),Other)],g)) /\
+  (known limit [Op t op xs] vs g =
+     let (ea1,g) = known limit xs vs g in
+     let (a,g) = known_op op (REVERSE (MAP SND ea1)) g in
      let e =
          if isGlobal op then
            dtcase gO_destApx a of
-               gO_None => Op t op (MAP FST e1)
+             | gO_None => Op t op (MAP FST ea1)
              | gO_Int i => Op t (Const i) []
              | gO_NullTuple tag => Op t (Cons tag) []
-         else Op t op (MAP FST e1)
+         else Op t op (MAP FST ea1)
      in
        ([(e,a)],g)) /\
-  (known [App t loc_opt x xs] vs g =
-     let (e2,g) = known xs vs g in
-     let (e1,g) = known [x] vs g in
-     let (e1,a1) = HD e1 in
-     let new_loc_opt =
-         dtcase loc_opt of
-           | SOME _ => loc_opt
-           | _ => dtcase dest_Clos a1 of
-                    | NONE => NONE
-                    | SOME (loc,arity) => if arity = LENGTH xs
-                                          then SOME loc else NONE
+  (known limit [App t loc_opt x xs] vs g =
+     let (ea2,g) = known limit xs vs g in
+     let (ea1,g) = known limit [x] vs g in
+     let (e1,a1) = HD ea1 in
+     let (new_loc_opt, body_opt) =
+         dtcase dest_Clos a1 of
+           | NONE => (loc_opt, NONE)
+           | SOME (loc,arity,body_opt) =>
+               if (loc_opt = NONE \/ loc_opt = SOME loc) /\ arity = LENGTH xs
+               then (SOME loc, body_opt)
+               else (loc_opt, NONE)
      in
-       ([(App t new_loc_opt e1 (MAP FST e2),Other)],g)) /\
-  (known [Fn t loc_opt ws_opt num_args x1] vs g =
-     let (e1,g) = known [x1] (REPLICATE num_args Other ++ vs) g in
-     let (body,a1) = HD e1 in
+       if SND limit = 0n then ([(App t new_loc_opt e1 (MAP FST ea2),Other)],g)
+       else
+       dtcase body_opt of
+          | NONE => ([(App t new_loc_opt e1 (MAP FST ea2),Other)],g)
+          | SOME body =>
+             if pure x then
+               let (eabody,_) = known (dec_depth limit) [body] (MAP SND ea2 ++ vs) g in
+               let (ebody,abody) = HD eabody
+               in
+                 ([(Let (t§0) (MAP FST ea2) (mk_Ticks t 1 (LENGTH xs) ebody),abody)],g)
+             else
+               let (eabody,_) = known (dec_depth limit) [body] (SNOC a1 (MAP SND ea2) ++ vs) g in
+               let (ebody,abody) = HD eabody
+               in
+                 ([(Let (t§0) (SNOC e1 (MAP FST ea2)) (mk_Ticks t 1 (LENGTH xs) ebody),abody)],g)) /\
+  (known limit [Fn t loc_opt ws_opt num_args x1] vs g =
+     let (ea1,g) = known limit [x1] (REPLICATE num_args Other ++ vs) g in
+     let (body,a1) = HD ea1 in
        ([(Fn t loc_opt NONE num_args body,
           dtcase loc_opt of
-          | SOME loc => Clos loc num_args
+          | SOME loc => clos_approx (size_limit limit) loc num_args body
           | NONE => Other)],g)) /\
-  (known [Letrec t loc_opt _ fns x1] vs g =
+  (known limit [Letrec t loc_opt _ fns x1] vs g =
      let clos = dtcase loc_opt of
                    NONE => REPLICATE (LENGTH fns) Other
-                |  SOME n => clos_gen n 0 fns in
+                |  SOME loc => clos_gen_noinline loc 0 fns in
      (* The following ignores SetGlobal within fns, but it shouldn't
         appear there, and missing it just means this opt will do less. *)
      let new_fns = MAP (\(num_args,x).
                     let new_vs = REPLICATE num_args Other ++ clos ++ vs in
-                    let res = known [x] new_vs g in
+                    let res = known limit [x] new_vs g in
                       (num_args,FST (HD (FST res)))) fns in
-     let (e1,g) = known [x1] (clos ++ vs) g in
-     let (e1,a1) = HD e1 in
+     let (ea1,g) = known limit [x1] (clos ++ vs) g in
+     let (e1,a1) = HD ea1 in
        ([(Letrec t loc_opt NONE new_fns e1,a1)],g))`
- (WF_REL_TAC `measure (exp3_size o FST)`
-  \\ REPEAT STRIP_TAC
-  \\ fs [GSYM NOT_LESS]
-  \\ IMP_RES_TAC EL_MEM_LEMMA
-  \\ IMP_RES_TAC exp1_size_lemma
-  \\ DECIDE_TAC);
+ (wf_rel_tac `inv_image (measure I LEX measure I)
+                        (\(limit, xs, vs, g). (depth_limit limit, exp3_size xs))`
+  \\ simp [dec_depth_def, depth_limit_def] \\ rpt strip_tac
+  \\ imp_res_tac exp1_size_lemma
+  \\ decide_tac);
+
+val known_ind = theorem "known_ind";
 
 val compile_def = Define `
   compile F exp = exp /\
   compile T exp =
-    let (_,g) = known [exp] [] LN in
-    let (e,_) = known [exp] [] g in
-      FST (HD e)`
+    let (_,g1) = known (0,0) [exp] [] LN in
+    let (e1,_) = known (0,0) [exp] [] g1 in
+    let (_,g2) = known (100,0) [FST (HD e1)] [] LN in
+    let (e2,_) = known (100,2) [FST (HD e1)] [] g2 in
+      FST (HD e2)`
 
 val known_LENGTH = Q.store_thm(
   "known_LENGTH",
-  `∀es vs g. LENGTH (FST (known es vs g)) = LENGTH es`,
-  ho_match_mp_tac (fetch "-" "known_ind") >> simp[known_def] >> rpt strip_tac >>
-  rpt (pairarg_tac >> fs[]))
+  `∀limit es vs g. LENGTH (FST (known limit es vs g)) = LENGTH es`,
+  recInduct known_ind >> simp[known_def] >> rpt strip_tac >>
+  rpt (pairarg_tac >> fs[]) >>
+  rw [] >> CASE_TAC >> CASE_TAC >> fs [] >>
+  rpt (pairarg_tac >> fs []));
 
 val known_LENGTH_EQ_E = Q.store_thm(
   "known_LENGTH_EQ_E",
-  `known es vs g0 = (alist, g) ⇒ LENGTH alist = LENGTH es`,
+  `known limit es vs g0 = (alist, g) ⇒ LENGTH alist = LENGTH es`,
   metis_tac[FST, known_LENGTH]);
 
 val known_sing = Q.store_thm(
   "known_sing",
-  `∀e vs g. ∃e' a g'. known [e] vs g = ([(e',a)], g')`,
-  rpt strip_tac >> Cases_on `known [e] vs g` >>
-  rename1 `known [e] vs g = (res,g')` >>
-  qspecl_then [`[e]`, `vs`, `g`] mp_tac known_LENGTH >> simp[] >>
+  `∀limit e vs g. ∃e' a g'. known limit [e] vs g = ([(e',a)], g')`,
+  rpt strip_tac >> Cases_on `known limit [e] vs g` >>
+  rename1 `known limit [e] vs g = (res,g')` >>
+  qspecl_then [`limit`, `[e]`, `vs`, `g`] mp_tac known_LENGTH >> simp[] >>
   Cases_on `res` >> simp[LENGTH_NIL] >> metis_tac[pair_CASES])
 
 val known_sing_EQ_E = Q.store_thm(
   "known_sing_EQ_E",
-  `∀e vs g0 all g. known [e] vs g0 = (all, g) ⇒ ∃e' apx. all = [(e',apx)]`,
+  `∀limit e vs g0 all g. known limit [e] vs g0 = (all, g) ⇒ ∃e' apx. all = [(e',apx)]`,
   metis_tac[PAIR_EQ, known_sing]);
 
+
 (*
+
+(* Trace starting points *)
+val t0 = ``SourceLoc 0 0 0 0``;
+val t1 = ``SourceLoc 1 1 1 1``;
+
+(* The numerical constant 1 *)
+val const1 = ``Op None (Const 1) []``;
+val const2 = ``Op None (Const 2) []``;
+
+
+(* fn f x => f x *)
+val apply = ``Fn None (SOME 0) NONE 2 (App ^t0 NONE (Var None 0) [Var None 1])``;
+
+(* fn x => x + 1 *)
+val succ = ``Fn None (SOME 2) NONE 1 (Op None Add [Var None 0; ^const1])``;
+
+(* -------------------------------*)
+
+(* (fn f x => f x) (fn x => x + 1) 2 *)
+val example_direct = ``App ^t1 NONE ^apply [^succ; ^const2]``;
+
+val inline_direct = ``clos_known$compile T ^example_direct``;
+EVAL inline_direct;
+
+val exp = ``Let None [^const1; ^const2] (Op None Add [Var None 0; Var None 1])`` 
+
+EVAL ``clos_letop$let_op [^exp]``;
+
+(*-------------------------------*)
+
+(*
+let apply = fn f x => f x
+    succ = fn x => x + 1
+in
+  apply succ 1
+end
+*)
+val example_local = ``Let None [^apply; ^succ] (App ^t1 NONE (Var None 0) [Var None 1; ^const1])``;
+val inlined_local = EVAL ``clos_known$compile T ^example_local``;
+
+val inline_local = ``clos_known$compile T ^example_local``;
+EVAL inline_local;
+
+(*-------------------------------*)
+
+(* fun apply <f,x> = f x *)
+val sg_apply = ``Op None (SetGlobal 0) [^apply]``;
+val g_apply = ``Op None (Global 0) []``;
+
+(* fun succ <x> = x + 1 *)
+val sg_succ = ``Op None (SetGlobal 1) [^succ]``;
+val g_succ = ``Op None (Global 1) []``;
+
+(*
+let _ = SetGlobal 0 (fn f x => f x)
+    _ = SetGlobal 1 (fn x => x + 1)
+in
+  (Global 0) (Global 1) 1
+end
+*)
+val example_global = ``Let None [^sg_apply; ^sg_succ] (App ^t1 NONE ^g_apply [^g_succ; ^const1])``;
+
+val inline_global = ``clos_known$compile T ^example_global``;
+
+EVAL inline_global;
+
+EVAL ``known (100,0) [^apply] [] LN``;
+EVAL ``known (100,0) [^succ] [] LN``;
+
+EVAL ``known (0,0) [^example_global] [] LN``;
+
+EVAL ``
+    let exp = ^example_local in
+    let (_,g1) = known (0,0) [exp] [] LN in
+    let (e1,g1') = known (0,0) [exp] [] g1 in
+    let (e2,g2) = known (0,0) [FST (HD e1)] [] LN in
+    (e1, e2, g1, g1')
+``
+
+
+    let (e2,_) = known (100,2) [FST (HD e1)] [] g2 in
+      FST (HD e2)
+
+*)
+
+(*
+
+  TEST 0.1
+
+  let
+    val f = fn k => 1
+  in f 6 end
+
+  val t = ``SourceLoc 0 0 0 0``
+  val f = ``Fn None (SOME 900) NONE 1 (Op None (Const 1) [])``
+  val exp = ``Let None [^f] (App ^t NONE (Var None 0) [Op None (Const 6) []])``
+
+  val ev = EVAL ``compile T ^exp``
+
+  TEST 0.2
+
+  let
+    val app = fn f x => f x
+    val f = fn x = x + 1
+  in app f 10 end
+
+  val t1 = ``SourceLoc 1 1 1 1``
+  val t2 = ``SourceLoc 2 2 2 2``
+  val app = ``Fn None (SOME 100) NONE 2 (App ^t1 NONE (Var None 0) [Var None 1])``
+  val f = ``Fn None (SOME 200) NONE 1 (Op None Add [Var None 0; Op None (Const 1) []])``
+  val exp = ``Let None [^app] (Let None [^f] (App ^t2 NONE (Var None 1) [Var None 0; Op None (Const 10) []]))``
+
+  val ev = EVAL ``compile T ^exp``
+
 
   TEST 1
 
   let fun f x = f x in f end
 
-  val f = ``Letrec (SOME 200) NONE [(1,App NONE (Var 1) [Var 0])] (Var 0)``
+  val f = ``Letrec None (SOME 200) NONE [(1,App None NONE (Var None 1) [Var None 0])] (Var None 0)``
   val ev = EVAL ``compile T ^f``
+
 
   TEST 2
 
@@ -324,9 +695,13 @@ val known_sing_EQ_E = Q.store_thm(
     val g = set_global 60 f
   in f 4 end
 
-  val f = ``Fn (SOME 900) NONE 1 (App NONE (Op (Global 60) []) [Op Add [Var 0; Op (Const 1) []]])``
-  val g = ``closLang$Op (SetGlobal 60) [Var 0]``
-  val exp = ``Let [^f] (Let [^g] (App NONE (Var 1) [Op (Const 4) []]))``
+  val t1 = ``SourceLoc 1 1 1 1``
+  val t2 = ``SourceLoc 2 2 2 2``
+  val f = ``Fn None (SOME 900) NONE 1 (App ^t1 NONE (Op None (Global 60) []) [Op None Add [Var None 0; Op None (Const 1) []]])``
+  val g = ``closLang$Op None (SetGlobal 60) [Var None 0]``
+  val exp = ``Let None [^f] (Let None [^g] (App ^t2 NONE (Var None 1) [Op None (Const 4) []]))``
+
+  val kn = EVAL ``(I ## sptree$toList) (known (100,2) [^exp] [] LN)``
   val ev = EVAL ``compile T ^exp``
 
   TEST 2A
@@ -338,11 +713,12 @@ val known_sing_EQ_E = Q.store_thm(
     get_global 60 3
   end
 
-  val f = ``Fn (SOME 900) NONE 1 (Op Add [Var 0; Op (Const 1) []])``
-  val g = ``closLang$Op (SetGlobal 60) [Var 0]``
-  val exp = ``Let [^f] (Let [^g] (App NONE
-                                      (Op (Global 60) [])
-                                      [Op (Const 3) []]))``
+  val t1 = ``SourceLoc 1 1 1 1``
+  val f = ``Fn None (SOME 900) NONE 1 (Op None Add [Var None 0; Op None (Const 1) []])``
+  val g = ``closLang$Op None (SetGlobal 60) [Var None 0]``
+  val exp = ``Let None [^f] (Let None [^g]
+                (App ^t1 NONE (Op None (Global 60) []) [Op None (Const 3) []]))``
+
   val ev = EVAL ``compile T ^exp``
 
 
@@ -356,10 +732,10 @@ val known_sing_EQ_E = Q.store_thm(
     h
   end
 
-  val h = ``closLang$Op (SetGlobal 62) [Op (Global 60) []]``
-  val exp = ``Let [^f] (Let [^g] (Let [^h] (Var 0)))``
+  val h = ``closLang$Op None (SetGlobal 62) [Op None (Global 60) []]``
+  val exp = ``Let None [^f] (Let None [^g] (Let None [^h] (Var None 0)))``
 
-  val ev1 = EVAL ``known [^exp] [] LN``
+  val ev1 = EVAL ``known (0, 0) [^exp] [] LN``
 
   TEST 2C
     (* is ghastly; the g-map will never pick up a good value for global 62 *)
@@ -372,13 +748,13 @@ val known_sing_EQ_E = Q.store_thm(
     h 1
   end
 
-  val h = ``Fn (SOME 800) NONE 1
-               (closLang$Op (SetGlobal 62) [Op (Global 60) []])``
-  val exp = ``Let [^f] (Let [^h]
-                (Let [^g] (App NONE (Var 1) [Op (Const 1) []])))``
+  val h = ``Fn None (SOME 800) NONE 1
+               (closLang$Op None (SetGlobal 62) [Op None (Global 60) []])``
+  val exp = ``Let None [^f] (Let None [^h]
+                (Let None [^g] (App None NONE (Var None 1) [Op None (Const 1) []])))``
 
-  val ev1 = EVAL ``known [^exp] [] LN``
-  val ev2 = EVAL ``known [^exp] [] ^(#2 (dest_pair (rhs (concl ev1))))``
+  val ev1 = EVAL ``known (0, 0) [^exp] [] LN``
+  val ev2 = EVAL ``known (0, 0) [^exp] [] ^(#2 (dest_pair (rhs (concl ev1))))``
 
 
   TEST 3
@@ -390,10 +766,12 @@ val known_sing_EQ_E = Q.store_thm(
   in #1 xy 4 end
 
 
-  val f = ``Fn (SOME 800) NONE 1 (Op Add [Var 0; Op (Const 1) []])``
-  val g = ``Fn (SOME 900) NONE 1 (Op Sub [Var 0; Op (Const 1) []])``
-  val xy = ``Let [^f;^g] (Op (Cons 0) [Var 0; Var 1])``
-  val app = ``Let [^xy] (App NONE (Op El [Var 0; Op (Const 0) []]) [Op (Const 4) []])``
+  val t = ``SourceLoc 0 0 0 0``
+  val f = ``Fn None (SOME 800) NONE 1 (Op None Add [Var None 0; Op None (Const 1) []])``
+  val g = ``Fn None (SOME 900) NONE 1 (Op None Sub [Var None 0; Op None (Const 1) []])``
+  val xy = ``Let None [^f;^g] (Op None (Cons 0) [Var None 0; Var None 1])``
+  val app = ``Let None [^xy] (App ^t NONE (Op None El [Op None (Const 0) []; Var None 0]) [Op None (Const 4) []])``
+
   val ev = EVAL ``compile T ^app``
 
 *)
